@prefix : <http://www.ontotext.com/proton/protontop#> .
@prefix dc: <http://purl.org/dc/elements/1.1/> .
@prefix owl: <http://www.w3.org/2002/07/owl#> .
@prefix rdf: <http://www.w3.org/1999/02/22-rdf-syntax-ns#> .
@prefix xml: <http://www.w3.org/XML/1998/namespace> .
@prefix xsd: <http://www.w3.org/2001/XMLSchema#> .
@prefix ptop: <http://www.ontotext.com/proton/protontop#> .
@prefix rdfs: <http://www.w3.org/2000/01/rdf-schema#> .
@base <http://www.ontotext.com/proton/protontop> .

<http://www.ontotext.com/proton/protontop> rdf:type owl:Ontology ;
                                            dc:title "Proton" ;
                                            owl:versionInfo "3.0" ;
                                            rdfs:label "Proton Ontology" ;
                                            dc:creator "Ontotext (Kiril Simov, Atanas Kiryakov, Ivan Terziev, Dimitar Manov, Mariana Damova, Svetoslav Petrov)" ;
                                            dc:rights "Proton ontology is available under the Creative Commons Attribution 3.0 Unported license; see http://creativecommons.org/licenses/by/3.0/. In a nutshell, you are free to copy, distribute and transmit the work; to remix/adapt the work (e.g. to import the ontology and create specializations of its elements), as long as you attribute the work in the manner specified by the author or licensor (but not in any way that suggests that they endorse you or your use of the work). Proper Attribution: Simply include the statement This work is based on Proton ontology, developed by Ontotext and link back to http://www.ontotext.com/proton-ontology" ;
                                            dc:subject "Upper-level ontology with extensions to handle Linked Open Data (LOD)" ;
                                            rdfs:comment "PROTON (Proto Ontology), Top module" .

#################################################################
#    Annotation properties
#################################################################

###  http://www.ontotext.com/proton/protontop#systemPrimitive
ptop:systemPrimitive rdf:type owl:AnnotationProperty ;
                     rdfs:comment "The system classes and properties are used to encode system specific information. They, as well as their instances and related information, should usually not be presented to the end-user. In practice, user-interface and visualization modules, can filter such primitives. All system primitives with this property should be marked with string value \"T\"."@en ;
                     rdfs:label "System Primitive"@en .


###  http://www.ontotext.com/proton/protontop#transitiveOver
ptop:transitiveOver rdf:type owl:AnnotationProperty ;
                    rdfs:comment "Makes possible the modelling of a specific, but rather useful modelling pattern. The semantics is defined with the following axiom: (p,transitiveOver,q) (x,p,y) (y,q,z) => (x,p,z). Sample usage is: (locatedIn, transitiveOver, subRegionOf) (Ontotext,locatedIn,Bulgaria) (Bulgaria,subRegionOf,Europe) => (Ontotext,locatedIn,Europe). The intended domain and range of this property are owl:ObjectProperty; those are not formally specified, in order not to get the ontology outside the OWL DL segment."@en ;
                    rdfs:label "Transitive over"@en .


###  http://www.w3.org/2000/01/rdf-schema#comment
rdfs:comment rdf:type owl:AnnotationProperty .


###  http://www.w3.org/2000/01/rdf-schema#label
rdfs:label rdf:type owl:AnnotationProperty .


###  http://www.w3.org/2002/07/owl#versionInfo
owl:versionInfo rdf:type owl:AnnotationProperty .


#################################################################
#    Object Properties
#################################################################

###  http://www.ontotext.com/proton/protontop#controls
ptop:controls rdf:type owl:ObjectProperty ;
              rdfs:subPropertyOf ptop:partiallyControls ;
              rdfs:comment "Indicates that an Agent has full control over an object. This is typically the case of wholly-owned subsidiaries and physicall possession of goods."@en ;
              rdfs:label "Controls"@en .


###  http://www.ontotext.com/proton/protontop#derivedFromSource
ptop:derivedFromSource rdf:type owl:ObjectProperty ;
                       rdfs:domain ptop:InformationResource ;
                       rdfs:range ptop:InformationResource ;
                       rdfs:comment "A reference to a resource from which the present resource is derived. The present resource may be derived from the Source resource in whole or in part. Recommended best practice is to identify the referenced resource by means of a string or number conforming to a formal identification system. DC2003ISO"@en ;
                       rdfs:label "Derived from Source"@en .


###  http://www.ontotext.com/proton/protontop#documentAuthor
ptop:documentAuthor rdf:type owl:ObjectProperty ;
                    rdfs:subPropertyOf ptop:hasCreator ;
                    rdfs:range ptop:Agent ;
                    rdfs:comment "The creator (or one of the creators) of a document."@en ;
                    rdfs:label "Document Author"@en .


###  http://www.ontotext.com/proton/protontop#establishedIn
ptop:establishedIn rdf:type owl:ObjectProperty ;
                   rdfs:subPropertyOf ptop:locatedIn ;
                   rdfs:domain ptop:Organization ;
                   rdfs:comment "The place where the organization is established or registered"@en ;
                   rdfs:label "Established in"@en .


###  http://www.ontotext.com/proton/protontop#hasChild
ptop:hasChild rdf:type owl:ObjectProperty ;
              rdfs:subPropertyOf ptop:hasRelative ;
              owl:inverseOf ptop:hasParent ;
              rdfs:comment "The relation of a parent to his/her child."@en ;
              rdfs:label "has Child"@en .


###  http://www.ontotext.com/proton/protontop#hasContactInfo
ptop:hasContactInfo rdf:type owl:ObjectProperty ;
                    rdfs:domain ptop:Object ;
                    rdfs:range ptop:ContactInformation ;
                    rdfs:comment "The information by which a given object can be contacted. Usually an address, telefon number, e-mail address, etc."@en ;
                    rdfs:label "has Contact Info"@en .


###  http://www.ontotext.com/proton/protontop#hasContributor
ptop:hasContributor rdf:type owl:ObjectProperty ;
                    rdfs:domain ptop:InformationResource ;
                    rdfs:range ptop:Agent ;
                    rdfs:comment "An agent responsible for making contributions to the content of a resource. Examples of Contributor include a person, an organization, or a service. DC2003ISO"@en ;
                    rdfs:label "has Contributor"@en .


###  http://www.ontotext.com/proton/protontop#hasCreator
ptop:hasCreator rdf:type owl:ObjectProperty ;
                rdfs:subPropertyOf ptop:hasContributor ;
                rdfs:comment "An agent primarily responsible for making the content of a resource. Examples of Creator include a person, an organization, or a service. Typically, the name of the Creator should be used to indicate the agent. (DC2003ISO, Creator)"@en ;
                rdfs:label "has Creator"@en .


###  http://www.ontotext.com/proton/protontop#hasEmployee
ptop:hasEmployee rdf:type owl:ObjectProperty ;
                 rdfs:subPropertyOf ptop:hasMember ;
                 rdfs:range ptop:Person ;
                 rdfs:comment "Relates a particular organization to its employees."@en ;
                 rdfs:label "has Employee"@en .


###  http://www.ontotext.com/proton/protontop#hasLeader
ptop:hasLeader rdf:type owl:ObjectProperty ;
               rdfs:subPropertyOf ptop:hasMember ;
               rdfs:range ptop:Person ;
               rdfs:comment "A general relation between an organization and a person who rules or guides or inspires it in some sense. It may or may not be an employee, may or may not be formal etc. Typically there is a single leader of an organization."@en ;
               rdfs:label "has Leader"@en .


###  http://www.ontotext.com/proton/protontop#hasMember
ptop:hasMember rdf:type owl:ObjectProperty ;
               rdfs:domain ptop:Group ;
               rdfs:range ptop:Agent ;
               rdfs:comment "Relates a particular organization to the agents that are its members. This predicate indicates `generic' membership, although there may be specialized kinds of membership in the same organization. Typically, membership eligibility is determined by the organization and accepted with the agent's voluntary affiliation. In many cases Persons that take Positions within Organization are considered members of the organization, although this is no way formally encoded here."@en ;
               rdfs:label "has Member"@en .


###  http://www.ontotext.com/proton/protontop#hasParent
ptop:hasParent rdf:type owl:ObjectProperty ;
               rdfs:subPropertyOf ptop:hasRelative ;
               rdfs:comment "Relation between a person and his/her mother or father."@en ;
               rdfs:label "has Parent"@en .


###  http://www.ontotext.com/proton/protontop#hasParticipant
ptop:hasParticipant rdf:type owl:ObjectProperty ;
                    rdfs:subPropertyOf ptop:hasParticipatingEntity ;
                    owl:inverseOf ptop:involvedIn ;
                    rdfs:domain ptop:Happening ;
                    rdfs:range ptop:Agent ;
                    rdfs:comment "The relation between a happenning and the agent involved in it. Fequently, the participants play some roles in the happening, then the appriate roles have to be introduced."@en ;
                    rdfs:label "Participant in a Happening"@en .


###  http://www.ontotext.com/proton/protontop#hasParticipatingEntity
ptop:hasParticipatingEntity rdf:type owl:ObjectProperty ;
                            owl:inverseOf ptop:involvedEntityIn ;
                            rdfs:domain ptop:Happening ;
                            rdfs:range ptop:Entity ;
                            rdfs:comment "The relation between a happening and an entity determining it. Such entities can be agents, instruments, materials, places, etc."@en ;
                            rdfs:label "Entity Participating in a Happening"@en .


###  http://www.ontotext.com/proton/protontop#hasPosition
ptop:hasPosition rdf:type owl:ObjectProperty ;
                 owl:inverseOf ptop:holder ;
                 rdfs:domain ptop:Person ;
                 rdfs:range ptop:JobPosition ;
                 rdfs:comment "Relation between a person and his/her job position."@en ;
                 rdfs:label "has Position"@en .


###  http://www.ontotext.com/proton/protontop#hasRelative
ptop:hasRelative rdf:type owl:ObjectProperty ,
                          owl:SymmetricProperty ;
                 rdfs:domain ptop:Person ;
                 rdfs:range ptop:Person ;
                 rdfs:comment "Relation between a person and his/her relatives - mother, father, brother, sister, child, etc."@en ;
                 rdfs:label "has Relative"@en .


###  http://www.ontotext.com/proton/protontop#hasSibling
ptop:hasSibling rdf:type owl:ObjectProperty ;
                rdfs:subPropertyOf ptop:hasRelative ;
                rdfs:comment "Relation between a person and his/her siblings - brother or sister."@en ;
                rdfs:label "has Sibling"@en .


###  http://www.ontotext.com/proton/protontop#hasSocialPosition
ptop:hasSocialPosition rdf:type owl:ObjectProperty ;
                       owl:inverseOf ptop:socialPositionHolder ;
                       rdfs:domain ptop:Person ;
                       rdfs:range ptop:SocialPosition ;
                       rdfs:comment "The relation between a person and the social position he has. "@en ;
                       rdfs:label "has Social Position"@en .


###  http://www.ontotext.com/proton/protontop#hasSpouse
ptop:hasSpouse rdf:type owl:ObjectProperty ;
               rdfs:subPropertyOf ptop:hasRelative ;
               rdf:type owl:SymmetricProperty ;
               rdfs:comment "Relation between a man and a woman that are married. This property is time constrained by the marriage happening for the two persons. Thus, one could have different spouses in different periods. If this time relation is important for a given domain, it needs to be modelled by the marriage happening."@en ;
               rdfs:label "has Spouse"@en .


###  http://www.ontotext.com/proton/protontop#hasSubject
ptop:hasSubject rdf:type owl:ObjectProperty ;
                rdfs:domain ptop:InformationResource ;
                rdfs:range ptop:Topic ;
                ptop:transitiveOver ptop:subTopicOf ;
                rdfs:comment "The topic of content of a given resource. Comment: Typically, the Subject will be expressed as keywords, key phrases, or classification codes that describe the topic of resource. Recommended best practice is to select a value from a controlled vocabulary or formal classification scheme. (DC2003ISO, Subject)"@en ;
                rdfs:label "has Subject"@en .


###  http://www.ontotext.com/proton/protontop#holder
ptop:holder rdf:type owl:ObjectProperty ;
            rdfs:domain ptop:JobPosition ;
            rdfs:range ptop:Person ;
            rdfs:comment "The person holding the position"@en ;
            rdfs:label "Holder"@en .


###  http://www.ontotext.com/proton/protontop#inLanguage
ptop:inLanguage rdf:type owl:ObjectProperty ;
                rdfs:domain ptop:InformationResource ;
                rdfs:range ptop:Language ;
                rdfs:comment "The language of the intellectual content of a resource. Recommended best practice is to use RFC 3066 [RFC3066], which, in conjunction with ISO 639 [ISO639], defines two- and three-letter primary language tags with optional subtags. Examples include “en” or “eng” for English, “akk” for Akkadian, and “en-GB” for English used in the United Kingdom. DC2003ISO"@en ;
                rdfs:label "in Language"@en .


###  http://www.ontotext.com/proton/protontop#involvedEntityIn
ptop:involvedEntityIn rdf:type owl:ObjectProperty ;
                      rdfs:domain ptop:Entity ;
                      rdfs:range ptop:Happening ;
                      rdfs:comment "The entities related to a given happening. Such entities can be agents, instruments, materials, places, etc."@en ;
                      rdfs:label "Entity Involved in"@en .


###  http://www.ontotext.com/proton/protontop#involvedIn
ptop:involvedIn rdf:type owl:ObjectProperty ;
                rdfs:subPropertyOf ptop:involvedEntityIn ;
                rdfs:domain ptop:Agent ,
                            ptop:Entity ;
                rdfs:range ptop:Happening ;
                rdfs:comment "The participating entities in a given happening that are agents. Participation is usually via some role."@en ;
                rdfs:label "Involved in"@en .


###  http://www.ontotext.com/proton/protontop#isBossOf
ptop:isBossOf rdf:type owl:ObjectProperty ;
              rdfs:domain ptop:Person ;
              rdfs:range ptop:Person ;
              rdfs:comment "Relates a Person to another one, where the first is the immediate boss or supervisor of the latter. This is a many-to-many relationship, i.e. there can be more than one boss of a person, even contemporally."@en ;
              rdfs:label "is Boss of"@en .


###  http://www.ontotext.com/proton/protontop#isOwnedBy
ptop:isOwnedBy rdf:type owl:ObjectProperty ;
               rdfs:domain ptop:Object ;
               rdfs:range ptop:Agent ;
               rdfs:comment "The relation between an object and an agent that is the owner of that object."@en ;
               rdfs:label "is Owned by"@en .


###  http://www.ontotext.com/proton/protontop#locatedIn
ptop:locatedIn rdf:type owl:ObjectProperty ,
                        owl:TransitiveProperty ;
               rdfs:domain ptop:Entity ;
               rdfs:range ptop:Location ;
               rdfs:comment "The relation between an object (also some happenings via their participants) and location where the object is."@en ;
               rdfs:label "Located in"@en .


###  http://www.ontotext.com/proton/protontop#operatedBy
ptop:operatedBy rdf:type owl:ObjectProperty ;
                rdfs:domain ptop:Service ;
                rdfs:range ptop:Agent ;
                rdfs:comment "A relation between a service and the agent (usually organisation), who provides it"@en ;
                rdfs:label "Operated by"@en .


###  http://www.ontotext.com/proton/protontop#owns
ptop:owns rdf:type owl:ObjectProperty ;
          rdfs:subPropertyOf ptop:partiallyOwns ;
          rdfs:comment "An agent fully owns an Object. In many cases this means also full control, unless the agent has transferred the control to another agent."@en ;
          rdfs:label "Owns"@en .


###  http://www.ontotext.com/proton/protontop#parentOrganizationOf
ptop:parentOrganizationOf rdf:type owl:ObjectProperty ;
                          rdfs:subPropertyOf ptop:partiallyControls ;
                          owl:inverseOf ptop:subsidiaryOrganizationOf ;
                          rdf:type owl:TransitiveProperty ;
                          rdfs:domain ptop:Organization ;
                          rdfs:range ptop:Organization ;
                          rdfs:comment "A relation between two organizations, where one of them is dependent on the other in some sense. This is a transitive relation, i.e. if organization X is a parent organization of Y and the latter is a parent organization of Z, then X is also considered a parent organization of Z. Inverse of subsidiaryOrganizationOf."@en ;
                          rdfs:label "Parent Organization of"@en .


###  http://www.ontotext.com/proton/protontop#partOf
ptop:partOf rdf:type owl:ObjectProperty ,
                     owl:TransitiveProperty ;
            rdfs:domain ptop:Entity ;
            rdfs:range ptop:Entity ;
            rdfs:comment "The general part-of relation which takes place between a whole and each of its parts. It has a number of specializations."@en ;
            rdfs:label "Part of"@en .


###  http://www.ontotext.com/proton/protontop#partiallyControls
ptop:partiallyControls rdf:type owl:ObjectProperty ;
                       rdfs:domain ptop:Agent ;
                       rdfs:range ptop:Object ;
                       rdfs:comment "Any sort of partial control an agent has with respect to an object."@en ;
                       rdfs:label "Partially Controls"@en .


###  http://www.ontotext.com/proton/protontop#partiallyOwns
ptop:partiallyOwns rdf:type owl:ObjectProperty ;
                   rdfs:subPropertyOf ptop:partiallyControls ;
                   rdfs:comment "Indicates that an Agent has some ownership over an object. It allows wide interpretations from \"I have a bike\" to \"John has shares in Fujitsu\"."@en ;
                   rdfs:label "Partially Owns"@en .


###  http://www.ontotext.com/proton/protontop#producedBy
ptop:producedBy rdf:type owl:ObjectProperty ;
                rdfs:domain ptop:ProductModel ;
                rdfs:range ptop:Agent ;
                rdfs:comment "A relation between a company and its ProductModel"@en ;
                rdfs:label "Produced by"@en .


###  http://www.ontotext.com/proton/protontop#registeredIn
ptop:registeredIn rdf:type owl:ObjectProperty ;
                  rdfs:subPropertyOf ptop:locatedIn ;
                  rdfs:domain ptop:Organization ;
                  rdfs:comment "A relation between an organization and the location in which it is registered."@en ;
                  rdfs:label "Registered in"@en .


###  http://www.ontotext.com/proton/protontop#roleHolder
ptop:roleHolder rdf:type owl:ObjectProperty ;
                rdfs:domain ptop:Role ;
                rdfs:range ptop:Entity ;
                rdfs:comment "The relation between a role and the entity that 'plays' a role in a given happening."@en ;
                rdfs:label "Role Holder"@en .


###  http://www.ontotext.com/proton/protontop#roleIn
ptop:roleIn rdf:type owl:ObjectProperty ;
            rdfs:domain ptop:Role ;
            rdfs:range ptop:Happening ;
            rdfs:comment "Relates a role to a happening, conditioned and affected by the role. Usually, the participants of a happening 'play' one or more roles in it."@en ;
            rdfs:label "Role in"@en .


###  http://www.ontotext.com/proton/protontop#socialPositionHolder
ptop:socialPositionHolder rdf:type owl:ObjectProperty ;
                          rdfs:domain ptop:SocialPosition ;
                          rdfs:range ptop:Person ;
                          rdfs:comment "The relation between a social position and the person who has it. "@en ;
                          rdfs:label "Social Position Holder"@en .


###  http://www.ontotext.com/proton/protontop#statedBy
ptop:statedBy rdf:type owl:ObjectProperty ;
              rdfs:domain ptop:Statement ;
              rdfs:range ptop:Agent ;
              rdfs:comment "Relates a statement to the agent who made it. In the case of an offer, the agent is the offerer; in case of a contract, those are the parties. In case of written statements, the creator/author and the \"stater\" could be different agents, due to the fact that one agent my have prepared and/or published a statement on behalf of another."@en ;
              rdfs:label "Stated by"@en .


###  http://www.ontotext.com/proton/protontop#subRegionOf
ptop:subRegionOf rdf:type owl:ObjectProperty ;
                 rdfs:subPropertyOf ptop:locatedIn ,
                                    ptop:partOf ;
                 rdf:type owl:TransitiveProperty ;
                 rdfs:domain ptop:Location ;
                 rdfs:comment "Relation between two locations where the first is contained within the other."@en ;
                 rdfs:label "Subregion of"@en .


###  http://www.ontotext.com/proton/protontop#subTopicOf
ptop:subTopicOf rdf:type owl:ObjectProperty ,
                         owl:TransitiveProperty ;
                rdfs:domain ptop:Topic ;
                rdfs:range ptop:Topic ;
                rdfs:comment "A relation from less general to more general topic. Defined to be transitive via rule."@en ;
                rdfs:label "Subtopic of"@en .


###  http://www.ontotext.com/proton/protontop#subsidiaryOrganizationOf
ptop:subsidiaryOrganizationOf rdf:type owl:ObjectProperty ;
                              rdfs:subPropertyOf ptop:partOf ;
                              rdfs:domain ptop:Organization ;
                              rdfs:range ptop:Organization ;
                              rdfs:comment "Indicates that an organization is in some sense part of another organization. This necessarily requires structural and organizational relations and may or may not indicate ownership. Its reverse, parentOrganizationOf, is a special case of partial control."@en ;
                              rdfs:label "Subsidiary Organization of"@en .


###  http://www.ontotext.com/proton/protontop#withinOrganization
ptop:withinOrganization rdf:type owl:ObjectProperty ;
                        rdfs:domain ptop:JobPosition ;
                        rdfs:range ptop:Organization ;
                        rdfs:comment "Determines in which organization is the position"@en ;
                        rdfs:label "within Organization"@en .


#################################################################
#    Data properties
#################################################################

###  http://www.ontotext.com/proton/protontop#description
ptop:description rdf:type owl:DatatypeProperty ;
                 rdfs:domain ptop:Entity ;
                 rdfs:comment "A textual description of an entity. Usually a free text in some natural language. As defined in DC2003ISO for InformationResources. In a sense, it is a specializatoin of rdf:comment"@en ;
                 rdfs:label "Description"@en .


###  http://www.ontotext.com/proton/protontop#documentAbstract
ptop:documentAbstract rdf:type owl:DatatypeProperty ;
                      rdfs:subPropertyOf ptop:description ;
                      rdfs:domain ptop:Document ;
                      rdfs:comment "An abstract or summary of a document."@en ;
                      rdfs:label "Document Abstract"@en .


###  http://www.ontotext.com/proton/protontop#documentSubTitle
ptop:documentSubTitle rdf:type owl:DatatypeProperty ;
                      rdfs:subPropertyOf ptop:laconicDescription ;
                      rdfs:domain ptop:Document ;
                      rdfs:comment "A very short sub-title of a document, usually a single sentence"@en ;
                      rdfs:label "Document Subtitle"@en .


###  http://www.ontotext.com/proton/protontop#doingBusinessAs
ptop:doingBusinessAs rdf:type owl:DatatypeProperty ;
                     rdfs:subPropertyOf ptop:name ;
                     rdfs:domain ptop:Organization ;
                     rdfs:comment "A name used for marketing purposes. Usually, it does not correspond to the legal name of the organisation."@en ;
                     rdfs:label "Doing Business as"@en .


###  http://www.ontotext.com/proton/protontop#endTime
ptop:endTime rdf:type owl:DatatypeProperty ;
             rdfs:domain ptop:Happening ;
             rdfs:comment "the end time point of a happening"@en ;
             rdfs:label "End Time"@en .


###  http://www.ontotext.com/proton/protontop#establishmentDate
ptop:establishmentDate rdf:type owl:DatatypeProperty ;
                       rdfs:domain ptop:Organization ;
                       rdfs:comment "The date when the organization was established or registered"@en ;
                       rdfs:label "Establishment Date"@en .


###  http://www.ontotext.com/proton/protontop#firstName
ptop:firstName rdf:type owl:DatatypeProperty ;
               rdfs:subPropertyOf ptop:name ;
               rdfs:domain ptop:Person ;
               rdfs:comment "The relation between a person and his/her first name. Usually used to call the person."@en ;
               rdfs:label "First Name"@en .


###  http://www.ontotext.com/proton/protontop#givenName
ptop:givenName rdf:type owl:DatatypeProperty ;
               rdfs:subPropertyOf ptop:name ;
               rdfs:domain ptop:Person ;
               rdfs:comment "The relation between a person and his/her given name."@en ;
               rdfs:label "Given Name"@en .


###  http://www.ontotext.com/proton/protontop#hasDate
ptop:hasDate rdf:type owl:DatatypeProperty ;
             rdfs:domain ptop:InformationResource ;
             rdfs:comment "Typically, Date will be associated with the creation or availability of the resource. Recommended best practice for encoding the date value is defined in a profile of ISO 8601 [W3CDTF] and includes (among others) dates of the form YYYY-MM-DD. For official documents, it could be the date of signature. It can also contain a java timestamp. Usually, time is connected to a happening (event/situation) in which the information resource is a participation entity. These include: creation of the information resource, its modification or other important happening. Very often such happening is in the background knowledge and the modeling of domain task does not require the explicit representation of this happening. If it plays important role in the model domain or for the task, then the user needs to extend the ontology in an appropriate way."@en ;
             rdfs:label "has Date"@en .


###  http://www.ontotext.com/proton/protontop#hasOldName
ptop:hasOldName rdf:type owl:DatatypeProperty ;
                rdfs:subPropertyOf ptop:name ;
                rdfs:comment "Relates an entity to its old name or alias that is no longer considered legitimate. For instance, Pekin is one of the old spellings of the name of the Chineese capital Beijing. The same happens to companies when they change their names and to womam when she gets married."@en ;
                rdfs:label "has Old Name"@en .


###  http://www.ontotext.com/proton/protontop#heldFrom
ptop:heldFrom rdf:type owl:DatatypeProperty ;
              rdfs:subPropertyOf ptop:startTime ;
              rdfs:domain ptop:JobPosition ;
              rdfs:comment "When the holder occupied a given position"@en ;
              rdfs:label "Held from"@en .


###  http://www.ontotext.com/proton/protontop#heldTo
ptop:heldTo rdf:type owl:DatatypeProperty ;
            rdfs:subPropertyOf ptop:endTime ;
            rdfs:domain ptop:JobPosition ;
            rdfs:comment "When the holder released a given position"@en ;
            rdfs:label "Held to"@en .


###  http://www.ontotext.com/proton/protontop#informationResourceCoverage
ptop:informationResourceCoverage rdf:type owl:DatatypeProperty ;
                                 rdfs:domain ptop:InformationResource ;
                                 rdfs:comment "The extent or scope of resource content. Typically, Coverage will include spatial location (a place name or geographic coordinates), temporal period (a period label, date, or date range), or jurisdiction (such as a named administrative entity). Recommended best practice is to select a value from a controlled vocabulary (for example, the Thesaurus of Geographic Names [TGN]) and to use, where appropriate, named places or time periods in preference to numeric identifiers such as sets of coordinates or date ranges. DC2003ISO"@en ;
                                 rdfs:label "Information Resource Coverage"@en .


###  http://www.ontotext.com/proton/protontop#informationResourceIdentifier
ptop:informationResourceIdentifier rdf:type owl:DatatypeProperty ;
                                   rdfs:domain ptop:InformationResource ;
                                   rdfs:comment "An unambiguous reference to the information resource within a given context. Recommended best practice is to identify the resource by means of a string or number conforming to a formal identification system. Formal identification systems include but are not limited to the Uniform Resource Identifier (URI) (including the Uniform Resource Locator (URL)), the Digital Object Identifier (DOI), and the International Standard Book Number (ISBN). DC2003ISO."@en ;
                                   rdfs:label "Information Resource Identifier"@en .


###  http://www.ontotext.com/proton/protontop#informationResourceRights
ptop:informationResourceRights rdf:type owl:DatatypeProperty ;
                               rdfs:domain ptop:InformationResource ;
                               rdfs:comment "Information about rights held in and over the resource. Typically, Rights will contain a rights management statement for the resource, or reference to a service providing such information. Rights information often encompasses Intellectual Property Rights (IPR), Copyright, and various Property Rights. If the Rights element is absent, no assumptions should be made about any rights held in or over the resource. DC2003ISO"@en ;
                               rdfs:label "Information Resource Rights"@en .


###  http://www.ontotext.com/proton/protontop#isLegalEntity
ptop:isLegalEntity rdf:type owl:DatatypeProperty ;
                   rdfs:domain ptop:Agent ;
                   rdfs:comment "Determines whether a particular Agent is a legal entity. The range should be constrained to Boolean. Agents, for which the value is True, correspond to instances of http://www.cyc.com/2003/04/01/cyc#LegalAgent, which is defined as follows \"Each instance of #LegalAgent is an agent who has some status in a particular legal system. At the very least, such an agent is recognized by some legal authority as having some kinds of rights and/or responsibilities as an agent (e.g., #citizens of Germany), ... \". In PROTON, it is modeled as property in order to avoid multiple-inheritance of classes and/or multiple classifications of instances."@en ;
                   rdfs:label "is Legal Entity"@en .


###  http://www.ontotext.com/proton/protontop#laconicDescription
ptop:laconicDescription rdf:type owl:DatatypeProperty ;
                        rdfs:subPropertyOf ptop:description ;
                        rdfs:comment "An extremely short (typically, single sentence) description of an entity"@en ;
                        rdfs:label "Laconic Description"@en .


###  http://www.ontotext.com/proton/protontop#lastName
ptop:lastName rdf:type owl:DatatypeProperty ;
              rdfs:subPropertyOf ptop:name ;
              rdfs:domain ptop:Person ;
              rdfs:comment "The relation between a person and his/her last name. Usually the family name."@en ;
              rdfs:label "Last Name"@en .


###  http://www.ontotext.com/proton/protontop#latitude
ptop:latitude rdf:type owl:DatatypeProperty ;
              rdfs:domain ptop:Location ;
              rdfs:comment "In degrees, minutes, and seconds: no sign or (+) = North; negative sign (-) = South."@en ;
              rdfs:label "Latitude"@en .


###  http://www.ontotext.com/proton/protontop#longitude
ptop:longitude rdf:type owl:DatatypeProperty ;
               rdfs:domain ptop:Location ;
               rdfs:comment "In degrees, minutes, and seconds: no sign or (+) = East; negative sign (-) = West."@en ;
               rdfs:label "Longitude"@en .


###  http://www.ontotext.com/proton/protontop#mainLabel
ptop:mainLabel rdf:type owl:DatatypeProperty ;
               rdfs:domain ptop:Entity ;
               rdfs:range rdfs:Literal ;
               rdfs:comment "This is a label of an entity which is consider to be representative for it. In cases when the entity is presented to someone, usually, this label will be used. In a sense, it is a specializatoin of rdfs:label"@en ;
               rdfs:label "Main Label"@en .


###  http://www.ontotext.com/proton/protontop#name
ptop:name rdf:type owl:DatatypeProperty ;
          rdfs:domain ptop:Entity ;
          rdfs:range rdfs:Literal ;
          rdfs:label "Name of any kind"@en .


###  http://www.ontotext.com/proton/protontop#nimaGNSDesignator
ptop:nimaGNSDesignator rdf:type owl:DatatypeProperty ;
                       rdfs:domain ptop:Location ;
                       rdfs:comment "The designator of the entity according to the NIMA GeoNames Server."@en ;
                       rdfs:label "NIMA GNS Designator"@en .


###  http://www.ontotext.com/proton/protontop#nimaGNSUniqueFeatureIndentifier
ptop:nimaGNSUniqueFeatureIndentifier rdf:type owl:DatatypeProperty ;
                                     rdfs:domain ptop:Location ;
                                     rdfs:comment "The Unique Feature Identifier from the NIMA GNS. A number which uniquely identifies the location."@en ;
                                     rdfs:label "NIMA GNS Unique Feature Identifier"@en .


###  http://www.ontotext.com/proton/protontop#numberOfEmployees
ptop:numberOfEmployees rdf:type owl:DatatypeProperty ;
                       rdfs:domain ptop:Organization ;
                       rdfs:comment "The estimated number of employees in the organization."@en ;
                       rdfs:label "Number of Employees"@en .


###  http://www.ontotext.com/proton/protontop#populationCount
ptop:populationCount rdf:type owl:DatatypeProperty ;
                     rdfs:domain ptop:Location ;
                     rdfs:comment "The number of citizens of a location."@en ;
                     rdfs:label "Population Count"@en .


###  http://www.ontotext.com/proton/protontop#resourceFormat
ptop:resourceFormat rdf:type owl:DatatypeProperty ;
                    rdfs:domain ptop:InformationResource ;
                    rdfs:comment "The physical or digital manifestation of the resource. Typically, Format will include the media-type or dimensions of the resource. Format may be used to identify the software, hardware, or other equipment needed to display or operate the resource. Examples of dimensions include size and duration. Recommended best practice is to select a value from a controlled vocabulary (for example, the list of Internet Media Types [MIME] defining computer media formats). DC2003ISO"@en ;
                    rdfs:label "Resource Format"@en .


###  http://www.ontotext.com/proton/protontop#resourceType
ptop:resourceType rdf:type owl:DatatypeProperty ;
                  rdfs:domain ptop:InformationResource ;
                  rdfs:comment "The nature or genre of the content of the resource. Type includes terms describing general categories, functions, genres, or aggregation levels for content. Recommended best practice is to select a value from a controlled vocabulary (for example, the DCMI Type Vocabulary [DCT]). To describe the physical or digital manifestation of the resource, use the resourceFormat property. DC2003ISO."@en ;
                  rdfs:label "Resource Type"@en .


###  http://www.ontotext.com/proton/protontop#startTime
ptop:startTime rdf:type owl:DatatypeProperty ;
               rdfs:domain ptop:Happening ;
               rdfs:comment "the starting moment of a happening"@en ;
               rdfs:label "Start Time"@en .


###  http://www.ontotext.com/proton/protontop#title
ptop:title rdf:type owl:DatatypeProperty ;
           rdfs:subPropertyOf ptop:name ;
           rdfs:domain ptop:InformationResource ;
           rdfs:comment "A name given to an information resource. Typically, title will be a name by which the resource is formally known. (DC2003ISO, Title there)"@en ;
           rdfs:label "Title"@en .


###  http://www.ontotext.com/proton/protontop#validFrom
ptop:validFrom rdf:type owl:DatatypeProperty ;
               rdfs:domain ptop:Statement ;
               rdfs:comment "The time when a statement is made valid. The happing of making the statement valid is not explicitly represented in Proton. If it is necessary for the task the ontology needs to be extented."@en ;
               rdfs:label "Valid from"@en .


###  http://www.ontotext.com/proton/protontop#validUntil
ptop:validUntil rdf:type owl:DatatypeProperty ;
                rdfs:domain ptop:Statement ;
                rdfs:comment "The time when a statement is made invalid. The happening of making the statement invalid is not explicitly represented in Proton. If it is necessary for the task the ontology should be extented."@en ;
                rdfs:label "Valid until"@en .


#################################################################
#    Classes
#################################################################

###  http://www.ontotext.com/proton/protontop#Abstract
ptop:Abstract rdf:type owl:Class ;
              rdfs:subClassOf ptop:Entity ;
              rdfs:comment "Something, which neither happens nor exists, e.g. a number or a chemical compound formula. Those are usually some symbols, invented to refer to general notions."@en ;
              rdfs:label "Abstract"@en .


###  http://www.ontotext.com/proton/protontop#Agent
ptop:Agent rdf:type owl:Class ;
           rdfs:subClassOf ptop:Object ;
           rdfs:comment "An Agent is something, which can show (carry out) an independent action, whether consciously or not. Most animals are considered agents, in most contexts; so are most organizations. According to DOLCE 2.0 \"objects to which we ascribe intentions, beliefs and desires\". In PROTON, Agent also denotes any automatic device and service, including web services and servers."@en ;
           rdfs:label "Agent"@en .


###  http://www.ontotext.com/proton/protontop#ContactInformation
ptop:ContactInformation rdf:type owl:Class ;
                        rdfs:subClassOf ptop:Abstract ;
                        rdfs:comment "Any instance of a particular notation, used to make the contact with an individual, an organization, or any other object possible."@en ;
                        rdfs:label "Contact Information"@en .


###  http://www.ontotext.com/proton/protontop#Document
ptop:Document rdf:type owl:Class ;
              rdfs:subClassOf ptop:InformationResource ;
              rdfs:comment "The information content of any sort of document. The tangible aspects are ignored. It is usually a document in free text with no formal structure or semantics."@en ;
              rdfs:label "Document"@en .


###  http://www.ontotext.com/proton/protontop#Entity
ptop:Entity rdf:type owl:Class ;
            rdfs:comment "Any sort of an entity of interest, usually something existing, happening, or purely abstract. Entities may have several - more than one - names or aliases."@en ;
            rdfs:label "Entity"@en .


###  http://www.ontotext.com/proton/protontop#Event
ptop:Event rdf:type owl:Class ;
           rdfs:subClassOf ptop:Happening ;
           rdfs:comment "A dynamic event, such as \"running\" or \"a concert\"."@en ;
           rdfs:label "Event"@en .


###  http://www.ontotext.com/proton/protontop#GeneralTerm
ptop:GeneralTerm rdf:type owl:Class ;
                 rdfs:subClassOf ptop:Abstract ;
                 rdfs:comment "General concept with well defined (idiomatic) meaning which can have a set of distinct lexical items (surface realizations) associated with it. Examples are: F2F, I18N, P2P, B2B, VIP, ASAP, Semantic Web"@en ;
                 rdfs:label "General Term"@en .


###  http://www.ontotext.com/proton/protontop#Group
ptop:Group rdf:type owl:Class ;
           rdfs:subClassOf ptop:Agent ;
           rdfs:comment "A group of agents that is not organized in any way. It could be the group of people in a bus or the shareholders of a company."@en ;
           rdfs:label "Group"@en .


###  http://www.ontotext.com/proton/protontop#Happening
ptop:Happening rdf:type owl:Class ;
               rdfs:subClassOf ptop:Entity ;
               rdfs:comment "Something that happens. It can be either dynamic - like in \"drawing a circle\", or static - like in \"being a president\". In all cases, a happening (an event, a situation, or a time period) has a certain (usually quite concrete) temporal positioning - in the simplest case it is the one, denoted by start and end point in time."@en ;
               rdfs:label "Happening"@en .


###  http://www.ontotext.com/proton/protontop#InformationResource
ptop:InformationResource rdf:type owl:Class ;
                         rdfs:subClassOf ptop:Statement ;
                         rdfs:comment "InformationResource denotes an information resource with identity, as defined in Dublin Core (DC2003ISO). InformationResource is considered any communication or message that is delivered or produced, taking into account the specific intention of its originator, and also the supposition (and anticipation) for a particular audience or counter-agent in the process of communication (i.e. passive or active feed-back)."@en ;
                         rdfs:label "Information Resource"@en .


###  http://www.ontotext.com/proton/protontop#JobPosition
ptop:JobPosition rdf:type owl:Class ;
                 rdfs:subClassOf ptop:SocialPosition ;
                 rdfs:comment "The situation of a person, holding a job (employment) position within an organization. The sub-classes of this class define a number of different types of positions."@en ;
                 rdfs:label "Job Position"@en .


###  http://www.ontotext.com/proton/protontop#Language
ptop:Language rdf:type owl:Class ;
              rdfs:subClassOf ptop:Abstract ;
              rdfs:comment "A spoken or written natural language"@en ;
              rdfs:label "Language"@en .


###  http://www.ontotext.com/proton/protontop#Location
ptop:Location rdf:type owl:Class ;
              rdfs:subClassOf ptop:Object ;
              rdfs:comment "Usually a geographic location on the earth, however any sort of 3D regions also fit here. The classification is based on the ADL Feature Type Thesaurus version 070203. Additionally, classes from Geonames classification are included. For each specific type, the corresponding NIMA GNS designators (DSG) are given."@en ;
              rdfs:label "Location"@en .


###  http://www.ontotext.com/proton/protontop#Number
ptop:Number rdf:type owl:Class ;
            rdfs:subClassOf ptop:Abstract ;
            rdfs:comment "Any given number, within the meaning that a number is one of the following: a concept of quantity derived from zero and units; or a numeral (or a string of numerals) used for identification (\"she refused to give them her Social Security number\"); or a phone number, etc."@en ;
            rdfs:label "Number"@en .


###  http://www.ontotext.com/proton/protontop#Object
ptop:Object rdf:type owl:Class ;
            rdfs:subClassOf ptop:Entity ;
            rdfs:comment "Objects are entities that could be claimed to exist - in some sense of existence. An object can play a certain role in some happenings. Objects could be substantially real - as the Buckingham Palace or a hardcopy book - or substantially imperceptible - for instance, an electronic document that exists only virtually, one cannot touch it."@en ;
            rdfs:label "Object"@en .


###  http://www.ontotext.com/proton/protontop#Organization
ptop:Organization rdf:type owl:Class ;
                  rdfs:subClassOf ptop:Group ;
                  rdfs:comment "Organization is a group, which is established in such a way that certain known relationships and obligations exist between the members, and/or between the organization and its members, and/or between the organization and the public (individuals or groups). It includes both informal and legally constituted organizations. Organizations can act as agents - to undertake projects, to enter into agreements, to own properties, etc. Most organizations have names. Almost all of them have at least two members."@en ;
                  rdfs:label "Organization"@en .


###  http://www.ontotext.com/proton/protontop#Person
ptop:Person rdf:type owl:Class ;
            rdfs:subClassOf ptop:Agent ;
            rdfs:comment "A Person is an agent, which is an individual who is a human being (i.e. any living or not alive member of the family Hominidae). Wordnet 2.0."@en ;
            rdfs:label "Person"@en .


###  http://www.ontotext.com/proton/protontop#ProductModel
ptop:ProductModel rdf:type owl:Class ;
                  rdfs:subClassOf ptop:Object ;
                  rdfs:comment "The general concept of a product model, for example, Ford T. The instances of this class are not specific instances of the product - the latter are just instances. Although product models are rather abstract entities (generally, intangible), this class is defined as a sub-class of Object, because it has a strong temporal extent (it comes to exsitence at some point of time). There could be several information resources associated with a product model (e.g. specifications, brouchures, etc.), but it is not an information resource on its own."@en ;
                  rdfs:label "Product Model"@en .


###  http://www.ontotext.com/proton/protontop#Role
ptop:Role rdf:type owl:Class ;
          rdfs:subClassOf ptop:Situation ;
          rdfs:comment "The role of an entity (usually an agent) within/during/affecting (intentionally or not) a particular happening. For instance a project coordinator, or a trial defendant, or even a material object that serves as an evidence in a trial (e.g. a weapon). Usually, we say 'this object is in this role in this happening'."@en ;
          rdfs:label "Role"@en .


###  http://www.ontotext.com/proton/protontop#Service
ptop:Service rdf:type owl:Class ;
             rdfs:subClassOf ptop:Object ;
             rdfs:comment "Any sort of service, ranging from a scheduled flight or train services to a weather forecast information/web serivce. Many services could be considered agents (usually software services)."@en ;
             rdfs:label "Service"@en .


###  http://www.ontotext.com/proton/protontop#Situation
ptop:Situation rdf:type owl:Class ;
               rdfs:subClassOf ptop:Happening ;
               rdfs:comment "A static event or situation, like \"sitting on a chair\" or \"holding position\". Typically, those are temporarily homogenous, i.e. their nature is not expected/required to change with their duration. As a happening, they used to happen/take place/be true for some periods of time and may or may not have a well-defined space extension."@en ;
               rdfs:label "Situation"@en .


###  http://www.ontotext.com/proton/protontop#SocialPosition
ptop:SocialPosition rdf:type owl:Class ;
                    rdfs:subClassOf ptop:Situation ;
                    rdfs:comment "The situation of a person, having a social position like celebrity, nobelty, job position, cleric, out of laws. The sub-classes of this class define different social statuses."@en ;
                    rdfs:label "Social Position"@en .


###  http://www.ontotext.com/proton/protontop#Statement
ptop:Statement rdf:type owl:Class ;
               rdfs:subClassOf ptop:Object ;
               rdfs:comment "A message that is stated or declared; a communication (oral or written), setting forth particulars or facts, etc; \"according to his statement he was in London on that day\". WordNet 1.7.1"@en ;
               rdfs:label "Statement"@en .


###  http://www.ontotext.com/proton/protontop#TimeInterval
ptop:TimeInterval rdf:type owl:Class ;
                  rdfs:subClassOf ptop:Happening ;
                  rdfs:comment "This is a general time expression, which refers to a particular period of time, an interval. Repeating periods (like Spring or Christmas) are not time intervals, while specific instances of them (like the Spring of 1944) are. A TimeInterval could collapse, in very special cases, to a time point, however in this case, in contrast to the Abstract time point (referring to some time during the day), it should be bound to a specific date, i.e. to represent a timestamp."@en ;
                  rdfs:label "Time Interval"@en .


###  http://www.ontotext.com/proton/protontop#Topic
ptop:Topic rdf:type owl:Class ;
           rdfs:subClassOf ptop:Abstract ;
           rdfs:comment "Any sort of a topic or theme, explicitly defined for classification purposes. As long as any other class or entity can play the role of a topic, the instances of this class are only those concepts that are defined to serve as topics. The topic class is the natural top-class for linkage of logically informal taxonomies."@en ;
           rdfs:label "Topic"@en .


###  Generated by the OWL API (version 4.2.6.20160910-2108) https://github.com/owlcs/owlapi
