# Saved by TopBraid on Wed Mar 10 12:12:47 EET 2010
# baseURI: http://proton.semanticweb.org/protons

@prefix :        <http://proton.semanticweb.org/protons#> .
@prefix owl:     <http://www.w3.org/2002/07/owl#> .
@prefix psys:    <http://proton.semanticweb.org/protons#> .
@prefix rdf:     <http://www.w3.org/1999/02/22-rdf-syntax-ns#> .
@prefix rdfs:    <http://www.w3.org/2000/01/rdf-schema#> .
@prefix xsd:     <http://www.w3.org/2001/XMLSchema#> .

<http://proton.semanticweb.org/protonsys>  ## it will be necessary to update
      rdf:type owl:Ontology ;
      rdfs:comment "PROTON (Proto Ontology), System module" ;
      owl:versionInfo "\"0.2\"" .

psys:description
      rdf:type owl:DatatypeProperty ;
      rdfs:comment "A textual description of an entity. Usually a free text in some natural language. As defined in DC2003ISO for InformationResources. In a sense, it is a specializatoin of rdf:comment" ;
      rdfs:domain psys:Entity ;
      rdfs:label "Description" .

psys:mainLabel
      rdf:type owl:DatatypeProperty ;
      rdfs:domain psys:Entity ;
      rdfs:label "main Label" ;
      rdfs:range rdfs:Literal ;
      rdfs:subPropertyOf rdfs:label .

psys:laconicDescription
      rdf:type owl:DatatypeProperty ;
      rdfs:comment "An extremely short (typically, single sentence) description of an entity  " ;
      rdfs:label "Laconic Description" ;
      rdfs:subPropertyOf psys:description .

psys:Recognized
      rdf:type owl:Class ;
      rdfs:comment "To identify a source (like a program or a module), which is capable of recognizing and generating new entities. Typically, those are not checked, and thus not trustable. An example for this is the NE-recognition process in KIM/GATE." ;
      rdfs:label "Recognized" ;
      rdfs:subClassOf psys:EntitySource ;
      psys:systemPrimitive
              "T" .
#############
## removed after a comment from KIM team on August, 24th 2010
#
#psys:Alias
#      rdf:type owl:Class ;
#      rdfs:comment "An alias of a named entity, usually not a general term but rather a name of something. Specific names, such as John and Smith, are not aliased on themselves. However, \"John Smith\" and \"Mr. Smith\" could be." ;
#      rdfs:label "Alias" ;
#      rdfs:subClassOf psys:LexicalResource ;
#      psys:systemPrimitive
#              "T" .
#
#psys:hasMainAlias
#      rdf:type owl:ObjectProperty ;
#      rdfs:comment "The official (or otherwise most important) alias of the entity" ;
#      rdfs:label "has Main Alias" ;
#      rdfs:subPropertyOf psys:hasAlias .
##############

psys:systemPrimitive
      rdf:type owl:AnnotationProperty ;
      rdfs:comment "The system classes and properties are used to encode system specific information. Those, as well as their instances and related information, should usually not be presented to the end-user. In practice, user-interface and visualization modules, can filter such primitives. All system primitives with this property should be marked with string value \"T\"." ;
      rdfs:label "System Primitive" .

psys:LexicalResource
      rdf:type owl:Class ;
      rdfs:comment "A lexical resource of any sort, usually part of a natural language or a specialized vocabulary. The rdf:label property defines the character string constituting the resource." ;
      rdfs:label "Lexical Resource" ;
      psys:systemPrimitive
              "T" .

psys:generatedBy
      rdf:type owl:ObjectProperty ;
      rdfs:comment "Identifies the party that introduced the entity into the KB." ;
      rdfs:domain psys:Entity ;
      rdfs:label "Generated by" ;
      rdfs:range psys:EntitySource ;
      psys:systemPrimitive
              "T" .

psys:transitiveOver
      rdf:type owl:AnnotationProperty ;
      rdfs:comment "Makes possible the modelling of a specific, but rather useful modelling pattern. The semantics is defined with the following axiom: (p,transitiveOver,q) (x,p,y) (y,q,z) => (x,p,z). Sample usage is: (locatedIn, transitiveOver, subRegionOf) (Ontotext,locatedIn,Bulgaria) (Bulgaria,subRegionOf,Europe) => (Ontotext,locatedIn,Europe). The intended domain and range of this property are owl:ObjectProperty; those are not formally specified, in order not to get the ontology outside the OWL DL segment." ;
      rdfs:label "Transitive over" .


psys:EntitySource
      rdf:type owl:Class ;
      rdfs:comment "A particular source where the entity (description) is derived/imported/extracted from. Can be used for maintenance of knowledge bases where information from multiple sources is being imported." ;
      rdfs:label "Entity Source" ;
      psys:systemPrimitive
              "T" .

psys:Trusted
      rdf:type owl:Class ;
      rdfs:comment "Used to indicate entities, imported from reliable (trusted) sources, like GNS, World Fact Book, GATE/MUSE/KIM gazetteers, but also any other trusted source." ;
      rdfs:label "Trusted" ;
      rdfs:subClassOf psys:EntitySource ;
      psys:systemPrimitive
              "T" .

psys:Entity
      rdf:type owl:Class ;
      rdfs:comment "Any sort of an entity of interest, usually something existing, happening, or purely abstract. Entities may have several - more than one - names or aliases." ;
      rdfs:label "Entity" .

psys:hasAlias
      rdf:type owl:ObjectProperty ;
      rdfs:domain psys:Entity ;
      rdfs:label "has Alias" ;
      rdfs:range psys:Alias .

